src/Fmajortofflatmajor.v
@@ -1,0 +1,353 @@
+Require Import compcert.lib.Coqlib.
+Require Import compcert.lib.Maps.
+Require Import compcert.lib.Integers.
+
+Require Import compcert.common.AST.
+Require Import compcert.common.Values.
+Require Import compcert.common.Globalenvs.
+Require Import compcert.common.Memory.
+Require Import compcert.common.Events.
+Require Import compcert.common.Switch.
+Require Import compcert.common.Smallstep.
+
+Require Import List.
+Import ListNotations.
+Require Import Arith.
+
+Require Import StructTact.StructTactics.
+Require Import StructTact.Util.
+
+Require Import HighValues.
+
+Require Import EricTact.
+
+Require Import Fmajor.
+Require Import Fflatmajor.
+
+
+Fixpoint transf_expr (f : Fmajor.expr) : Fflatmajor.expr :=
+  match f with
+  | Fmajor.Var id => Var id
+  | Fmajor.Deref e n => Deref (transf_expr e) n
+  end.
+
+Fixpoint transf_stmt (s : Fmajor.stmt) : Fflatmajor.stmt :=
+  let fix transf_cases (cases : list (Z * Fmajor.stmt)) :=
+      match cases with
+      | (z,s) :: cases' => (z,transf_stmt s) :: transf_cases cases'
+      | nil => nil
+      end in
+  match s with
+  | Fmajor.Sskip => Sskip
+  | Fmajor.Scall dst fn arg => Scall dst (transf_expr fn) (transf_expr arg)
+  | Fmajor.Sassign dst exp => Sassign dst (transf_expr exp)
+  | Fmajor.SmakeConstr dst tag args => SmakeConstr dst tag (map transf_expr args)
+  | Fmajor.SmakeClose dst fname args => SmakeClose dst fname (map transf_expr args) 
+  | Fmajor.Sseq s1 s2 => Sseq (transf_stmt s1) (transf_stmt s2)
+  | Fmajor.Sswitch targid cases target => Fflatmajor.Sswitch targid (transf_cases cases) (transf_expr target)
+  end.
+
+Fixpoint transf_cases (cases : list (Z * Fmajor.stmt)) :=
+  match cases with
+  | (z,s) :: cases' => (z,transf_stmt s) :: transf_cases cases'
+  | nil => nil
+  end.
+
+Definition transf_fun_body (f : (Fmajor.stmt * Fmajor.expr)) : Fflatmajor.stmt :=
+  let (s,e) := f in
+  Sseq (transf_stmt s) (Sreturn (transf_expr e)).
+
+Definition transf_fundef (f : Fmajor.function) : Fflatmajor.fundef :=
+  Fflatmajor.mkfunction (Fmajor.fn_params f) (Fmajor.fn_sig f) (Fmajor.fn_stackspace f)
+                    (transf_fun_body (Fmajor.fn_body f)).
+                    
+Definition transf_program (p : Fmajor.program) : Fflatmajor.program :=
+  AST.transform_program transf_fundef p.
+
+
+Section PRESERVATION.
+
+Variable prog: Fmajor.program.
+Variable tprog: Fflatmajor.program.
+Let ge := Genv.globalenv prog.
+Let tge := Genv.globalenv tprog.
+Hypothesis TRANSF : transf_program prog = tprog.
+
+(* The Fflatmajor continuation will have a lot more going on *)
+(* It could have arbitrarily many Kblocks stuck in whenever *)
+(* Somewhere we need to record more precise info *)
+
+Inductive match_cont: Fmajor.cont -> Fflatmajor.cont -> Prop :=
+| match_stop :
+    match_cont Fmajor.Kstop Fflatmajor.Kstop
+| match_switch : forall k k',
+    match_cont k k' ->
+    match_cont (Fmajor.Kswitch k) (Fflatmajor.Kswitch k')
+| match_return :
+    forall k k' exp,
+      match_cont k k' ->
+      match_cont (Fmajor.Kreturn exp k) (Fflatmajor.Kseq (Sreturn (transf_expr exp)) k')
+| match_seq :
+    forall k k' s s',
+      match_cont k k' ->
+      transf_stmt s = s' ->
+      match_cont (Fmajor.Kseq s k) (Fflatmajor.Kseq s' k')
+| match_call :
+    forall id f env k k' exp,
+      match_cont k k' ->
+      match_cont (Fmajor.Kcall id exp f env k) (Fflatmajor.Kcall id (transf_fundef f) env k').
+
+Inductive match_states: Fmajor.state -> Fflatmajor.state -> Prop :=
+| match_state :
+    forall f f' s s' k k' e env,
+      transf_fundef f = f' ->
+      transf_stmt s = s' ->
+      match_cont k k' ->
+      match_states (Fmajor.State f s e k env) (Fflatmajor.State f' s' k' env)
+| match_returnstate :
+    forall v k k',
+      match_cont k k' ->
+      match_states (Fmajor.Returnstate v k) (Fflatmajor.Returnstate v k').
+
+Lemma eval_expr_transf :
+  forall env exp v,
+    Fmajor.eval_expr env exp v ->
+    Fflatmajor.eval_expr env (transf_expr exp) v.
+Proof.
+  induction 1; intros.
+  simpl. econstructor; eauto.
+  econstructor; eauto.
+  eapply eval_deref_constr; eauto.
+Qed.
+
+Lemma eval_exprlist_transf :
+  forall env expl vs,
+    Fmajor.eval_exprlist env expl vs ->
+    Fflatmajor.eval_exprlist env (map transf_expr expl) vs.
+Proof.
+  induction 1; intros;
+    econstructor; eauto.
+  eapply eval_expr_transf; eauto.
+Qed.
+
+Lemma find_symbol_transf :
+  forall id b,
+    Genv.find_symbol ge id = Some b ->
+    Genv.find_symbol tge id = Some b.
+Proof.
+  intros.
+  unfold ge in *. unfold tge in *.
+  subst tprog. unfold transf_program.
+  erewrite Genv.find_symbol_transf; eauto.
+Qed.
+
+Lemma find_funct_ptr_transf :
+  forall b f,
+    Genv.find_funct_ptr ge b = Some f ->
+    Genv.find_funct_ptr tge b = Some (transf_fundef f).
+Proof.
+  intros.
+  unfold ge in *. unfold tge in *.
+  subst tprog. unfold transf_program.
+  erewrite Genv.find_funct_ptr_transf; eauto.
+Qed.
+
+
+Lemma find_case_transf :
+  forall cases z s,
+    Fmajor.find_case z cases = Some s ->
+    find_case z (transf_cases cases) = Some (transf_stmt s).
+Proof.
+  induction cases; intros.
+  simpl in *. inv H.
+  simpl in *.
+  break_match_hyp. subst a.
+  break_match_hyp. subst.
+  simpl. rewrite zeq_true. congruence.
+  simpl. rewrite zeq_false by congruence.
+  eapply IHcases; eauto.
+Qed.
+
+Lemma step_sim_nil_trace :
+  forall (s1 s1' : Fmajor.state) (s2 : Fflatmajor.state),
+    match_states s1 s2 ->
+    Fmajor.step ge s1 E0 s1' ->
+    exists s2',
+      plus Fflatmajor.step tge s2 E0 s2' /\ match_states s1' s2'.
+Proof.
+  intros.
+  inversion H; inversion H0; remember tprog; subst;
+  repeat match goal with
+             | [ H : Fmajor.State _ _ _ _ _ = Fmajor.State _ _ _ _ _ |- _ ] => inversion H; remember tprog; subst
+  end; try congruence.
+  (* assign stmt *)
+  + eexists. split. eapply plus_one.
+    
+    econstructor; eauto.
+    eapply eval_expr_transf; eauto.
+    econstructor; eauto.
+
+  (* skip/seq *)
+  + (* What we need: *)
+    (* k' is some kind of Kseq *)
+
+    invp match_cont.
+    eexists. split. eapply plus_one.
+    econstructor; eauto.
+    econstructor; eauto.
+
+    
+    
+  (* skip/return *)
+  + destruct k0; simpl in H6;
+      try solve [inv H6].
+    (* Kstop case: end of program return *)
+    inv H3. inv H5.
+    app eval_expr_transf Fmajor.eval_expr.
+    eexists. split. eapply plus_left; nil_trace.
+    simpl.
+    econstructor; eauto.
+    eapply star_one.
+    econstructor; eauto.
+    econstructor; eauto.
+
+    
+    (* Kcall case: end of function *)
+    inv H3. inv H5.
+    app eval_expr_transf Fmajor.eval_expr.
+    eexists. split. eapply plus_left; nil_trace.
+    simpl.
+    econstructor; eauto.
+    eapply star_one.
+    econstructor; eauto.
+    econstructor; eauto.
+
+  (* scall to callstate *)
+  + app eval_expr_transf (Fmajor.eval_expr env earg).
+    app eval_expr_transf (Fmajor.eval_expr env efunc).
+    destruct (Fmajor.fn_body fn) eqn:?.
+    eexists. split.
+    eapply plus_left; nil_trace.
+    simpl. econstructor; eauto.
+    eapply find_symbol_transf; eauto.
+    eapply find_funct_ptr_transf; eauto.
+    simpl. find_rewrite. reflexivity.
+    simpl. rewrite H11. reflexivity.
+    eapply star_left; nil_trace.
+    econstructor; eauto.
+    eapply star_one.
+    simpl. unfold transf_fun_body.
+    find_rewrite.
+    eapply step_seq.
+
+    econstructor; eauto.
+    
+    simpl.
+    econstructor; eauto.
+    econstructor; eauto.
+
+  (* seq *)
+  + eexists. split.
+    eapply plus_one. simpl.
+    econstructor.
+    econstructor; eauto.
+    econstructor; eauto.
+
+  (* make_constr *)
+  + eexists. split.
+    eapply plus_one.
+    econstructor; eauto.
+    eapply eval_exprlist_transf; eauto.
+    econstructor; eauto.
+
+  (* make_close *)
+  + eexists. split.
+    eapply plus_one.
+    econstructor; eauto.
+    eapply eval_exprlist_transf; eauto.
+    eapply find_symbol_transf; eauto.
+    eapply find_funct_ptr_transf; eauto.
+    econstructor; eauto.
+
+  (* switch *)
+  + app eval_expr_transf Fmajor.eval_expr.
+    eexists. split.
+    eapply plus_one.
+    simpl. fold transf_cases. econstructor; eauto.
+    eapply find_case_transf; eauto.
+    econstructor; eauto.
+    econstructor; eauto.
+
+  (* kswitch *)
+  + inv H3.
+    eexists; split.
+    eapply plus_one.
+    econstructor; eauto.
+    econstructor; eauto.
+    
+  (* Returnstate *)
+  + inv H5.
+    invp match_cont.
+    
+    eexists. split.
+    eapply plus_one.
+    econstructor; eauto.
+    econstructor; eauto.
+Qed.    
+
+Lemma step_sim :
+  forall (s1 s1' : Fmajor.state) (s2 : Fflatmajor.state) t,
+    match_states s1 s2 ->
+    Fmajor.step ge s1 t s1' ->
+    exists s2',
+      plus Fflatmajor.step tge s2 t s2' /\ match_states s1' s2'.
+Proof.
+  intros.
+  assert (t = E0) by (inv H0; congruence).
+  subst t.
+  eapply step_sim_nil_trace; eauto.
+Qed.
+
+(* maybe don't need? *)
+Lemma initial_states_match :
+  forall s1,
+    Fmajor.initial_state prog s1 ->
+    exists s2, Fflatmajor.initial_state tprog s2 /\ match_states s1 s2.
+Proof.
+  intros.
+  inv H. eexists; split.
+  econstructor; eauto.
+  unfold transf_program.
+  erewrite Genv.find_symbol_transf; eauto.
+  unfold transf_program.
+  erewrite Genv.find_funct_ptr_transf; eauto.
+  econstructor; eauto.
+
+  
+Admitted.
+
+
+Lemma match_final_states :
+  forall s1 s2 r,
+    match_states s1 s2 ->
+    Fmajor.final_state s1 r ->
+    Fflatmajor.final_state s2 r.
+Proof.
+Admitted.
+
+Theorem fsim :
+  forward_simulation (Fmajor.semantics prog) (Fflatmajor.semantics tprog).
+Proof.
+  eapply forward_simulation_plus.
+  intros. simpl.
+  unfold transf_program in *. subst tprog.
+  solve [eapply Genv.public_symbol_transf].
+
+  solve [eapply initial_states_match; eauto].
+  solve [eapply match_final_states; eauto].
+
+  intros. eapply step_sim; eauto.
+  
+Qed.
+  
+End PRESERVATION.
